\documentclass[../ana1u.tex]{subfiles}
\begin{document}
\setcounter{section}{11}
\section{(01.02.19)}
\begin{defi}
    Die Funktion \( \abb{f}{I}{\R} \) hat in \( x_0 \in I \) die Ableitung \(a \in \R \),
    falls 
    \[\limesx{x}{x_0} \frac{f(x) - f(x_0)}{x-x_0} = a \]
    Alternativ:
    \[f'(x_0) = a \Leftrightarrow \limesx{h}{0} \frac{f(x_0+h)-f(x_0)}{h} = a \] 
\end{defi}
\begin{bsp}
    \begin{beh}
        \(\abb{f}{\R}{\R} \) ist differenzierbar in allen \(x_0 \in \R \) mit Ableitung 
        \(f'(x_0) = e^{x_0} \)
    \end{beh}
    \begin{bew}
        Sei \(x_0 \in \R \) beliebig aber fest
        \[\phi(h) = \frac{e^{x_0+h}-e^{x_0}}{h} = \frac{e^{x_0}e^{h}-e^{x_0}}{h}
        = e^{x_0} \cdot \frac{e^{h} - 1}{h}\]
        z.z. \(\limesx{x}{0} \frac{e^{x}-1}{x} = 1 \) \\
        FÃ¼r \(x \neq 0 \) gilt:
        \[\frac{e^{x}-1}{x} = \frac{1}{x} \left(\sum_{k=0}^{\infty} \frac{x^k}{k!} - 1\right)
        = \left(\sum_{k=0}^{\infty} \frac{x^{k-1}}{k!}\right) := P(x) \]  
        Die Potenzreihe \(P(x) \) ist stetig in \(x\)
        \[\limesx{x}{0} P(x) = P(0) = 1\]
        somit folgt:
        \[\limesx{h}{0} \phi(h) = \limesx{h}{0} e^{x_0} \cdot \frac{e^h - 1}{h} 
        = e^{x_0} \cdot \limesx{h}{0} \frac{e^h-1}{h} = e^{x_0} \Rightarrow f'(x_0) = e^{x_0}\]
    \end{bew}
\end{bsp}
\begin{bsp}
    \begin{beh}
        \(\abb{f}{\R}{\R}: x \mapsto \sin(x) \) ist differenzierbar in allen \(x_0 \in \R \)
        und \(f'(x_0) = \cos(x_0) \) 
    \end{beh}
    \begin{bew}
        Sei \(x_0 \in \R \) beliebig aber fest
    \end{bew}
\end{bsp}
\end{document}